books/coi/generalize/generalize.lisp
@@ -1,0 +1,540 @@
+#|-*-Lisp-*-=================================================================|#
+#|                                                                           |#
+#| coi: Computational Object Inference                                       |#
+#|                                                                           |#
+#|===========================================================================|#
+(in-package "ACL2")
+
+;;
+;; A generic generalization routine
+;;
+
+(include-book "coi/symbol-fns/symbol-fns" :dir :system)
+(include-book "coi/util/mv-nth" :dir :system)
+(include-book "coi/gensym/gensym" :dir :system)
+
+(local (include-book "coi/bags/top" :dir :system))
+(local (include-book "coi/lists/set" :dir :system))
+
+;; You may wrap terms that you wish to generalize with the
+;; function (gensym::generalize term)
+
+(defun gensym::generalize (x) x)
+
+(defevaluator gensym::eval gensym::eval-list
+  (
+   (if a b c)
+   (gensym::generalize x)
+   )
+  )
+
+(in-theory (disable GENSYM::EVAL-CONSTRAINT-6))
+(in-theory (disable GENSYM::EVAL-CONSTRAINT-7))
+
+(defun pattern-match-rec (args terms alist)
+  (declare (type (satisfies alistp) alist)
+	   (xargs :verify-guards nil))
+  (if (and (consp args)
+	   (consp terms))
+      (met ((hit alist)
+	    (let ((pattern (car args))
+		  (term    (car terms)))
+	      (cond
+	       ((symbolp pattern)
+		(let ((hit (assoc pattern alist)))
+		  (if (consp hit)
+		      (if (equal (cdr hit) term)
+			  (mv t alist)
+			(mv nil nil))
+		    (mv t (cons (cons pattern term) alist)))))
+	       ((consp pattern)
+		(cond
+		 ((and (consp term) (not (equal (car term) 'quote)))
+		  (let ((pfn   (car pattern))
+			(pargs (cdr pattern))
+			(tfn   (car term))
+			(targs (cdr term)))
+		    (if (equal pfn tfn)
+			(pattern-match-rec pargs targs alist)
+		      (mv nil nil))))
+		 (t (mv nil nil))))
+	       (t
+		(mv nil nil)))))
+	(if hit (pattern-match-rec (cdr args) (cdr terms) alist)
+	  (mv nil nil)))
+    (if (and (null args) (null terms))
+	(mv t alist)
+      (mv nil nil))))
+
+(defthm alistp-pattern-match-rec
+  (implies
+   (alistp alist)
+   (alistp (v1 (pattern-match-rec args terms alist)))))
+
+(verify-guards pattern-match-rec)
+
+(defun clause-keys (clauses)
+  (declare (type t clauses)
+	   (xargs :Verify-guards nil))
+  (if (consp clauses)
+      (let ((clause (car clauses)))
+	(cond
+	 ((symbolp clause)
+	  (cons clause (clause-keys (cdr clauses))))
+	 ((atom clause)
+	  (clause-keys (cdr clauses)))
+	 ((eq (car clause) 'quote)
+	  (clause-keys (cdr clauses)))
+	 ((consp (car clause))
+	  (append (clause-keys (cdr clause))
+		  (clause-keys (cdr clauses))))
+	 (t
+	  (append (clause-keys (cdr clause))
+		  (clause-keys (cdr clauses))))))
+    nil))
+
+(defthm true-listp-clause-keys
+  (true-listp (clause-keys clauses)))
+
+(verify-guards clause-keys)
+
+(defthm not-member-key-clause-keys-reduction
+  (implies
+   (and
+    (consp a)
+    (pseudo-term-listp clauses)
+    (not (bag::memberp (caar a) (clause-keys clauses))))
+   (equal (gensym::eval-list clauses a)
+	  (gensym::eval-list clauses (cdr a))))
+  :hints (("Goal" :in-theory (enable PSEUDO-TERMP pseudo-term-listp)
+	   :induct (clause-keys clauses))
+	  (and stable-under-simplificationp
+	       '(:in-theory (enable GENSYM::EVAL-CONSTRAINT-0)))))
+
+(defun term-keys (term)
+  (declare (type t term))
+  (cond
+   ((symbolp term)
+    (list term))
+   ((atom term)
+    nil)
+   ((eq (car term) 'quote)
+    nil)
+   ((consp (car term))
+    (clause-keys (cdr term)))
+   (t
+    (clause-keys (cdr term)))))
+
+(defthm not-member-key-term-keys-reduction
+  (implies
+   (and
+    (consp a)
+    (pseudo-termp term)
+    (not (bag::memberp (caar a) (term-keys term))))
+   (equal (gensym::eval term a)
+	  (gensym::eval term (cdr a))))
+  :hints (("Goal" :in-theory (enable GENSYM::EVAL-CONSTRAINT-0 pseudo-termp))))
+
+(in-theory (disable term-keys))
+
+(defun pattern-match-list (list terms)
+  (declare (type t list terms))
+  (if (and (consp list) (consp (car list)))
+      (let ((pattern (caar list))
+	    (type-p  (cdar list)))
+	(met ((hit alist) (pattern-match-rec pattern terms nil))
+	     (declare (ignore alist))
+	     (if hit (mv terms type-p)
+	       (pattern-match-list (cdr list) terms))))
+    (mv nil nil)))
+
+(defun pattern-match-args (fn args terms)
+  (declare (type t fn args terms))
+  (if (consp terms)
+      (let ((term (car terms)))
+	(cond
+	 ((atom term)
+	  (pattern-match-args fn args (cdr terms)))
+	 ((eq (car term) 'quote)
+	  (pattern-match-args fn args (cdr terms)))
+	 ((consp (car term))
+	  (or
+	   (pattern-match-args fn args (cdr term))
+	   (pattern-match-args fn args (cdr terms))))
+	 (t
+	  (or (and (equal fn (car term))
+		   (met ((subterm type-p) (pattern-match-list args (cdr term)))
+			(and subterm (cons (cons fn subterm) type-p))))
+	      (pattern-match-args fn args (cdr term))
+	      (pattern-match-args fn args (cdr terms))))))
+    nil))
+
+#+joe
+(defthm pseudo-termp-pattern-match
+  (implies
+   (pseudo-term-listp terms)
+   (pseudo-termp (pattern-match-args fn args terms))))
+
+(defun replace-common-subterm (subterm var terms)
+  (declare (type t subterm var terms))
+  (if (consp terms)
+      (let ((term (car terms)))
+	(if (equal term subterm)
+	    (cons var (replace-common-subterm subterm var (cdr terms)))
+	  (cond
+	   ((atom term)
+	    (cons term (replace-common-subterm subterm var (cdr terms))))
+	   ((eq (car term) 'quote)
+	    (cons term (replace-common-subterm subterm var (cdr terms))))
+	   ((consp (car term))
+	    (cons (cons (car term) (replace-common-subterm subterm var (cdr term)))
+		  (replace-common-subterm subterm var (cdr terms))))
+	   (t
+	    (cons (cons (car term) (replace-common-subterm subterm var (cdr term)))
+		  (replace-common-subterm subterm var (cdr terms)))))))
+    nil))
+
+(defthm len-replace-common-subterm
+  (equal (len (replace-common-subterm suterm var list))
+	 (len list)))
+
+(defthm pseudo-termp-listp-replace-common-subterm
+  (implies 
+   (and
+    (pseudo-termp var)
+    (pseudo-term-listp clauses))
+   (pseudo-term-listp (replace-common-subterm subterm var clauses)))
+  :hints (("Goal" :in-theory (enable pseudo-termp
+				     pseudo-term-listp))))
+
+(defthm generic-replace-common-subterm-reduction
+  (implies
+   (and
+    var
+    (symbolp var)
+    (equal (cdr (assoc-eq var a)) (gensym::eval subterm a)))
+   (equal (gensym::eval-list (replace-common-subterm subterm var terms) a)
+	  (gensym::eval-list terms a)))
+  :hints ((and stable-under-simplificationp
+	       '(:in-theory (enable GENSYM::EVAL-CONSTRAINT-0)))
+	  ("Goal" :induct (replace-common-subterm subterm var terms))))
+
+(local
+ (defthm non-membership-from-non-memberp-superset-free
+   (implies
+    (and
+     (not (list::memberp a x))
+     (list::subsetp y x))
+    (not (list::memberp a y))))
+ )
+
+(local
+ (defthm subsetp-term-append-term
+   (list::subsetp term (append term x)))
+ )
+
+(local
+ (defthm subsetp-x-append-term-x
+   (list::subsetp x (append term x)))
+ )
+
+(defun generalization-symbol-base (subterm)
+  (declare (type t subterm))
+  (if (and (consp subterm)
+	   (consp (cdr subterm))
+	   (consp (cadr subterm)))
+      (let ((symbol (caadr subterm)))
+	(if (symbolp symbol) symbol `gensym::||))
+    `gensym::||))
+
+(defun generalize-clause-processor (clause subterm)
+  (declare (type t clause subterm))
+  (if (consp subterm)
+      (let ((fn (generalization-symbol-base subterm)))
+	(let ((avoid (append (term-keys subterm) (clause-keys clause))))
+	  (let ((var (gensym::gensym fn avoid)))
+	    (if (not var) (mv nil nil)
+	      (mv var (replace-common-subterm subterm var clause))))))
+    (mv nil nil)))
+
+(defun generalize-clause-alist (clause a subterm)
+  (declare (type t clause subterm))
+  (if (consp subterm)
+      (let ((fn (generalization-symbol-base subterm)))
+	(let ((avoid (append (term-keys subterm) (clause-keys clause))))
+	  (let ((var (gensym::gensym fn avoid)))
+	    (if (not var) a
+	      (cons (cons var (gensym::eval subterm a)) a)))))
+    a))
+
+(defthm eval-v0-generalize-clause-processor
+  (implies
+   (and
+    (v0 (generalize-clause-processor clause subterm))
+    (pseudo-termp subterm))
+   (equal (gensym::eval (v0 (generalize-clause-processor clause subterm)) (GENERALIZE-CLAUSE-ALIST clause A subterm))
+	  (gensym::eval subterm a))))
+
+(defthm eval-subterm-GENERALIZE-CLAUSE-ALIST
+  (implies
+   (and
+    (v0 (generalize-clause-processor clause subterm))
+    (pseudo-termp subterm)
+    (pseudo-termp term)
+    (list::subsetp (term-keys term) (append (term-keys subterm) (clause-keys clause))))
+   (equal (gensym::eval term (GENERALIZE-CLAUSE-ALIST clause A subterm))
+	  (gensym::eval term a)))
+  :hints (("Goal" :in-theory (disable LIST::SUBSETP-APPEND-2))))
+
+
+(defthm generalize-clause-processor-reduction
+  (implies
+   (and
+    (pseudo-term-listp clause)
+    (pseudo-termp subterm)
+    (v0 (generalize-clause-processor clause subterm)))
+   (equal (gensym::eval-list (v1 (generalize-clause-processor clause subterm))
+			     (generalize-clause-alist clause a subterm))
+	  (gensym::eval-list clause a))))
+  
+(defthm generalize-clause-alist-reduction
+  (implies
+   (and
+    (pseudo-term-listp clause)
+    (pseudo-termp subterm))
+   (equal (gensym::eval-list clause (generalize-clause-alist clause a subterm))
+	  (gensym::eval-list clause a))))
+  
+(in-theory (disable generalize-clause-processor generalize-clause-alist))
+
+(in-theory (enable GENSYM::EVAL-CONSTRAINT-6))
+(in-theory (enable GENSYM::EVAL-CONSTRAINT-7))
+
+(include-book "coi/util/clause-processor" :dir :system)
+
+;;(conjoin-disjoin gensym::eval gensym::eval-list)
+(clause-eval-facts gensym::eval gensym::eval-list)
+
+(defthmd disjoin-congruence
+  (implies
+   (equal (gensym::eval-list args1 a1) 
+	  (gensym::eval-list args2 a2))
+   (iff (iff (gensym::eval (disjoin args1) a1)
+	     (gensym::eval (disjoin args2) a2)) t))
+  :hints (("Goal" :expand ((disjoin args2)
+			   (disjoin args1))
+	   :induct (list::len-len-induction args1 args2))))
+
+;;
+;; This may be generally useful .. push back into clause-processor?
+;;
+
+(defthm disjoin-implication
+  (implies
+   (and
+    (equal (gensym::eval-list args1 a1)
+	   (gensym::eval-list args2 a2))
+    (gensym::eval (disjoin args1) a1))
+   (gensym::eval (disjoin args2) a2))
+  :hints (("Goal" :use disjoin-congruence)))
+
+#|
+(defthm disjoin2-congruence-1
+  (implies
+   (and
+    (gensym::eval (disjoin2 w x) a1)
+    (iff (gensym::eval w a1) (gensym::eval y a2))
+    (iff (gensym::eval x a1) (gensym::eval z a2)))
+   (gensym::eval (disjoin2 y z) a2)))
+
+(defthm disjoin2-congruence-2
+  (implies
+   (and
+    (not (gensym::eval (disjoin2 w x) a1))
+    (iff (gensym::eval w a1) (gensym::eval y a2))
+    (iff (gensym::eval x a1) (gensym::eval z a2)))
+   (not (gensym::eval (disjoin2 y z) a2))))
+
+(local (in-theory (disable disjoin2)))
+
+(defthm disjoin2-ite-reduction
+  (implies
+   (and
+    (consp ite)
+    (equal (car ite) 'if))
+   (iff (gensym::eval (disjoin2 ite x) a)
+	(if (gensym::eval (cadr ite) a)
+	    (gensym::eval (disjoin2 (caddr ite) x) a)
+	  (gensym::eval (disjoin2 (cadddr ite) x) a))))
+  :hints (("Goal" :in-theory (enable disjoin2))))
+
+(in-theory (disable conjoin2))
+
+(defthm eval-conjoin2
+  (iff (gensym::eval (conjoin2 x y) a)
+       (and (gensym::eval x a)
+	    (gensym::eval y a)))
+  :hints (("Goal" :in-theory (enable conjoin2))))
+
+(defthm eval-disjoin2
+  (iff (gensym::eval (disjoin2 x y) a)
+       (or (gensym::eval x a)
+	   (gensym::eval y a)))
+  :hints (("Goal" :in-theory (enable disjoin2))))
+|#
+
+(defun generalize-termp (term)
+  (declare (type t term))
+  (and (pseudo-termp term)
+       (consp term)
+       (consp (cdr term))
+       (null (cddr term))
+       (equal (car term) 'gensym::generalize)))
+
+(defun generalize-clause-processor-wrapper (clause hint)
+  (declare (type t clause hint))
+  (if (consp hint)
+      (let ((subterm (car hint))
+	    (type-p  (cdr hint)))
+	(met ((var new) (generalize-clause-processor clause subterm))
+	     (if (and (generalize-termp subterm) (symbolp type-p) (not (equal type-p 'quote)) var)
+		 (if type-p
+		     (list
+		      (cons `(if (,type-p ,(cadr subterm)) ,*t* ,*nil*) new)
+		      (cons `(if (,type-p ,var) ,*nil* ,*t*) new)
+		      )
+		   (list new))
+	       (list clause))))
+    (list clause)))
+
+(defun generalize-clause-alist-wrapper (clause a hint)
+  (declare (type t clause hint))
+  (if (consp hint)
+      (let ((subterm (car hint))
+	    (type-p  (cdr hint)))
+	(met ((var new) (generalize-clause-processor clause subterm))
+	     (declare (ignore new))
+	     (if (and (generalize-termp subterm) (symbolp type-p) (not (equal type-p 'quote)) var) 
+		 (generalize-clause-alist clause a subterm)
+	       a)))
+    a))
+
+(defthm term-keys-generalize-termp
+  (implies
+   (generalize-termp subterm)
+   (equal (term-keys subterm)
+	  (clause-keys (cdr subterm))))
+  :hints (("Goal" :in-theory (enable CLAUSE-KEYS term-keys))))
+
+(defthm open-clause-keys
+  (implies
+   (and
+    (syntaxp (not (symbolp terms)))
+    (consp terms))
+   (equal (clause-keys terms)
+	  (append (term-keys (car terms))
+		  (clause-keys (cdr terms)))))
+  :hints (("Goal" :in-theory (enable term-keys clause-keys))))
+
+(defthm clause-keys-null
+  (implies
+   (not (consp terms))
+   (equal (clause-keys terms) nil))
+  :hints (("Goal" :in-theory (enable term-keys clause-keys))))
+
+
+(defthm generalize-clause-processor-works
+  (implies
+   (and
+    (pseudo-term-listp cl)
+    (alistp a)
+    (gensym::eval (conjoin-clauses (generalize-clause-processor-wrapper cl hint))
+	      (generalize-clause-alist-wrapper cl a hint)))
+   (gensym::eval (disjoin cl) a))
+  :hints (("Goal" :do-not-induct t
+	   :do-not '(eliminate-destructors generalize)
+	   :in-theory (e/d (pseudo-termp pseudo-term-listp GENSYM::EVAL-CONSTRAINT-0)
+			   (LIST::SUBSETP-APPEND-2))
+	   :use ((:instance disjoin-implication
+			    (args1 cl)
+			    (a1    (generalize-clause-alist cl a (car hint)))
+			    (args2 cl)
+			    (a2    a))
+		 (:instance disjoin-implication
+			    (args1 (val 1 (generalize-clause-processor cl (car hint))))
+			    (a1    (generalize-clause-alist cl a (car hint)))
+			    (args2 cl)
+			    (a2    a)))))
+  :rule-classes :clause-processor)
+
+(defun get-generalization-patterns (world)
+  (declare (xargs :guard (and (worldp world)
+                              (alistp (table-alist 'generalization world)))))
+  (cdr (assoc-eq :patterns (table-alist 'generalization world))))
+
+(defun generalize-pattern-hint (patterns clause)
+  (declare (xargs :mode :program))
+  (let ((hint (pattern-match-args 'gensym::generalize patterns clause)))
+    (and hint
+	 (let ((hints `(:clause-processor (generalize-clause-processor-wrapper clause ',hint))))
+	   `(:computed-hint-replacement 
+	     ((generalize-clause-hint id clause world))
+	     ,@hints)))))
+
+(defun generalize-clause-hint (id clause world)
+  (declare (xargs :mode :program)
+	   (ignore id))
+  (or (generalize-pattern-hint (get-generalization-patterns world) clause)
+      nil))
+
+(add-default-hints!
+ '((generalize-clause-hint id clause world)))
+
+(defmacro add-generalization-pattern (pattern &key (type 'nil))
+  `(table generalization :patterns
+	  (cons ',(cons `(,pattern) type)
+		(cdr (assoc :patterns (table-alist 'generalization world))))))
+
+;; Can we add a fixing function to the mix?  Create a new symbol and apply the
+;; fixing function?
+;;
+;;(add-generalization-pattern (foo x y z) :type fix)
+
+(in-theory (disable gensym::generalize))
+
+(encapsulate
+ ()
+(local
+(encapsulate
+ ()
+
+ (defun foo (x) x)
+ (defun goo (x)
+   (declare (ignore x))
+   t)
+
+ (defthm open-goo
+   (implies
+    (and
+     (syntaxp (symbolp x))
+     (integerp x))
+    (goo x)))
+
+ (in-theory (disable goo (:type-prescription goo)))
+
+ (defthm integerp-foo
+   (implies
+    (integerp x)
+    (integerp (foo x))))
+
+ (in-theory (disable foo (:type-prescription foo)))
+
+ (add-generalization-pattern (foo x) :type integerp)
+
+ ;; This works only because of the generalization of (foo x)
+ (defthm pred-foo
+   (implies
+    (integerp x)
+    (goo (gensym::generalize (foo x)))))
+
+ )))
